clean up sugar

src/Pipit.System.Exp.fst
@@ -1,7 +1,6 @@
 (* Translation to transition system *)
 module Pipit.System.Exp
 
-(*SHELVED: use Pipit.Norm.System
 open Pipit.Prim.Table
 open Pipit.Exp.Base
 module Causal = Pipit.Exp.Causality
@@ -15,7 +14,7 @@ open Pipit.System.Det
 (* A system we get from translating an expression *)
 let xsystem (#t: table) (c: context t) (state: Type) (value: Type) = system (row c) state value
 (* Same, but deterministic *)
-let xdsystem (#t: table) (c: context t) (state: Type) (value: Type) = dsystem (row c) state value
+// let xdsystem (#t: table) (c: context t) (state: Type) (value: Type) = dsystem (row c) state value
 
 let xsystem_stepn
   (#tbl: table)
@@ -26,24 +25,71 @@ let xsystem_stepn
   (s': state): prop =
   system_stepn t streams s'
 
-let rec state_of_exp (#t: table) (#c: context t) (e: exp t c 'a): Tot Type (decreases e) =
+let rec state_of_exp (#t: table) (#c: context t) (#a: t.ty) (e: exp t c a): Tot Type (decreases e) =
   match e with
-  | XVal v -> unit
-  | XPrim p -> unit
-  | XBVar x -> unit
-  | XVar x -> unit
-  | XApp f e -> state_of_exp f & state_of_exp e
-  | XFby v e1 -> state_of_exp e1 & 'a
-  | XThen e1 e2 -> system_then_state (state_of_exp e1) (state_of_exp e2)
+  | XBase _ -> unit
+  | XApps e1 -> state_of_exp_apps e1
+  | XFby v e1 -> state_of_exp e1 & t.ty_sem a
   | XMu e1 -> state_of_exp e1
   | XLet b e1 e2 -> state_of_exp e1 & state_of_exp e2
-  // Contracts do not expose their body, so we only need state of assumptions, guarantee and arg
-  // | XContract assm guar body arg ->
-  //   state_of_exp assm &
-  //   state_of_exp guar &
-  //   state_of_exp arg
-  | XCheck name e1 e2 -> (t.ty_sem t.propty & state_of_exp e1) & state_of_exp e2
+  | XCheck name e1 -> (t.ty_sem t.propty & state_of_exp e1)
+  // Contracts do not expose their body in abstract mode, so we only need state of rely and guar
+  | XContract rely guar impl ->
+    state_of_exp rely & state_of_exp guar
 
+and state_of_exp_apps (#t: table) (#c: context t) (#a: funty t.ty) (e: exp_apps t c a): Tot Type (decreases e) =
+  match e with
+  | XPrim _ -> unit
+  | XApp f e -> state_of_exp_apps f & state_of_exp e
+
+let rec system_of_exp
+  (#t: table) (#c: context t) (#a: t.ty)
+  (e: exp t c a { Causal.causal e }):
+    Tot (xsystem c (state_of_exp e) (t.ty_sem a)) (decreases e) =
+  // if exp_is_function e then system_of_dsystem (dsystem_of_exp e)
+  // else
+    match e with
+    | XBase (XVal v) -> system_const v
+    | XBase (XBVar x) -> system_map (fun i -> CR.index (context_sem c) i x) system_input
+    | XBase (XVar x) -> false_elim ()
+    | XApps e1 -> system_of_exp_apps e1
+    | XFby v e1 ->
+      system_pre v (system_of_exp e1)
+    | XMu e1 ->
+      let t' = system_of_exp e1 in
+      system_mu #(row c) #(t.ty_sem a & row c) (fun i v -> (v, i)) t'
+    | XLet b e1 e2 ->
+      system_let (fun i v -> (v, i)) (system_of_exp e1) (system_of_exp e2)
+    // | XContract assm guar body arg ->
+    //   system_contract_instance (fun i b -> (b, ())) (fun i a b -> (a, (b, ())))
+    //     (system_bool_holds (system_of_exp assm))
+    //     (system_bool_holds (system_of_exp guar))
+    //     (system_of_exp arg)
+    | XCheck name e1 ->
+      system_check t.propty_sem (t.propty_of_bool true) name (system_of_exp e1)
+    | XContract rely guar impl ->
+      admit ()
+
+and system_of_exp_apps
+  (#t: table) (#c: context t) (#a: funty t.ty)
+  (e: exp_apps t c a { Causal.causal_apps e }):
+    Tot (xsystem c (state_of_exp_apps e) (funty_sem t.ty_sem a)) (decreases e) =
+  // if exp_is_function e then system_of_dsystem (dsystem_of_exp e)
+  // else
+    match e with
+    | XPrim p -> system_const (t.prim_sem p)
+    | XApp e1 e2 ->
+      let arg = XApp?.arg e in
+      let ret = XApp?.ret e in
+      lemma_funty_sem_FTFun t.ty_sem (XApp?.arg e) (XApp?.ret e);
+      // assert_norm (Causal.causal_ (XApp e1 e2) ==> (Causal.causal e1 && Causal.causal e2));
+      let t1: xsystem c _ (funty_sem t.ty_sem (FTFun arg ret)) = system_of_exp_apps e1 in
+      let t2: xsystem c _ (t.ty_sem arg) = system_of_exp e2 in
+      system_ap2 t1 t2
+      // let t': xsystem c (state_of_exp_apps (XApp e1 e2)) (funty_sem t.ty_sem a) = system_ap2 t1 t2 in
+
+
+(*
 let rec dsystem_of_exp (#t: table) (#c: context t) (e: exp t c 'a { Causal.causal e }):
     Tot (xdsystem c (state_of_exp e) 'a) (decreases e) =
   match e with
@@ -71,44 +117,4 @@ let rec dsystem_of_exp (#t: table) (#c: context t) (e: exp t c 'a { Causal.causa
     let t2 = dsystem_of_exp e2 in
     let t': xdsystem c (state_of_exp (XCheck name e1 e2)) 'a = dsystem_let (fun i v -> i) t1 t2 in
     t'
-
-let rec system_of_exp_rel
-  (#t: table) (#c: context t)
-  (e: exp t c 'a { Causal.causal e }):
-    Tot (xsystem c (state_of_exp e) 'a) (decreases e) =
-  // if exp_is_function e then system_of_dsystem (dsystem_of_exp e)
-  // else
-    match e with
-    | XVal v -> system_const v
-    | XPrim p -> system_const (t.prim_sem p)
-    | XBVar x -> system_map (fun i -> CR.index (context_sem c) i x) system_input
-    | XVar x -> false_elim ()
-    | XApp e1 e2 ->
-      assert_norm (Causal.causal (XApp e1 e2) ==> (Causal.causal e1 && Causal.causal e2));
-      let t1 = system_of_exp_rel e1 in
-      let t2 = system_of_exp_rel e2 in
-      let t': xsystem c (state_of_exp (XApp e1 e2)) 'a = system_ap2 t1 t2 in
-      t'
-    | XFby v e1 ->
-      system_pre v (system_of_exp_rel e1)
-    | XThen e1 e2 ->
-      system_then (system_of_exp_rel e1) (system_of_exp_rel e2)
-    | XMu e1 ->
-      let t' = system_of_exp_rel e1 in
-      system_mu #(row c) #('a & row c) (fun i v -> (v, i)) t'
-    | XLet b e1 e2 ->
-      system_let (fun i v -> (v, i)) (system_of_exp_rel e1) (system_of_exp_rel e2)
-    // | XContract assm guar body arg ->
-    //   system_contract_instance (fun i b -> (b, ())) (fun i a b -> (a, (b, ())))
-    //     (system_bool_holds (system_of_exp_rel assm))
-    //     (system_bool_holds (system_of_exp_rel guar))
-    //     (system_of_exp_rel arg)
-    | XCheck name e1 e2 ->
-      let t1 = system_check t.propty_sem (t.propty_of_bool true) name (system_of_exp_rel e1) in
-      let t2 = system_of_exp_rel e2 in
-      let t': xsystem c (state_of_exp (XCheck name e1 e2)) 'a = system_let (fun i v -> i) t1 t2 in
-      t'
-
-let system_of_exp (#t: table) (#c: context t) (e: exp t c 'a { Causal.causal e }) =
-  system_of_dsystem (dsystem_of_exp e)
 *)
